.

theories/System/STLC.v
@@ -12,8 +12,6 @@ Export ChurchStyleStlc.
 Notation "Gamma '∋' x '⦂' A" := (Lookup x A Gamma) : type_scope.
 Notation "Gamma '⊢' M '⦂' A" := (Typing Gamma M A) : type_scope.
 Notation "Gamma '⊢' M '=' N '⦂' A" := (equality Gamma M N A) : type_scope.
-Notation "Gamma '⊢' M '⇉' A" := (typNe Gamma M A) : type_scope.
-Notation "Gamma '⊢' M '⇇' A" := (typNf Gamma M A) : type_scope.
 
 Section STLC_META.
 
@@ -53,21 +51,64 @@ Lemma substTyping_Typing {Gamma : ctx L} {e : trm L} {ty : typ L} {s : subst L} 
 Proof.
 Admitted.
 
-Section Soundness_of_NbE.
+Section WEAK_NORMALISATION.
 
-Fixpoint interpret_typ (Gamma : ctx L) (ty : typ L) {struct ty} : eval_typ Gamma ty -> trm L -> Prop :=
-  match ty as ty return eval_typ Gamma ty -> trm L -> Prop with
-  | bty _ b => fun d : B.sig (trm L) (fun u => typNe Gamma u (bty _ b)) => fun e : trm L =>
-    Gamma ⊢ d.(B.proj1_sig) = e ⦂ bty _ b
-  | (ty1 -> ty2)%typ => fun d : forall Gamma' : ctx L, le_ctx Gamma Gamma' -> eval_typ Gamma' ty1 -> eval_typ Gamma' ty2 => fun e1 : trm L =>
-    forall Gamma' : ctx L, forall LE : le_ctx Gamma Gamma', forall a : eval_typ Gamma' ty1, forall e2 : trm L, interpret_typ Gamma' ty1 a e2 -> interpret_typ Gamma' ty2 (d Gamma' LE a) (App_trm e1 e2)
+Inductive typNe (Gamma : ctx L) : trm L -> typ L -> Prop :=
+  | typNe_Var x ty
+    (LOOKUP : Lookup x ty Gamma)
+    : typNe Gamma (Var_trm x) ty
+  | typNe_App u v ty ty'
+    (u_typNe : typNe Gamma u (ty -> ty')%typ)
+    (v_typNf : typNf Gamma v ty)
+    : typNe Gamma (App_trm u v) ty'
+  | typNe_Con c ty
+    (ty_eq : ty = Sigma c)
+    : typNe Gamma (Con_trm c) ty
+  where "Gamma '⊢' M '⇉' A" := (typNe Gamma M A)
+with typNf (Gamma : ctx L) : trm L -> typ L -> Prop :=
+  | typNf_of_typNe u v ty
+    (u_typNe : typNe Gamma u ty)
+    (ALPHA : alphaEquiv v u)
+    : typNf Gamma v ty
+  | typNf_Lam x v ty ty'
+    (v_typNf : typNf ((x, ty) :: Gamma) v ty')
+    : typNf Gamma (Lam_trm x ty v) (ty -> ty')%typ
+  | typNf_beta_typNf v v' ty
+    (BETA : betaOnce v v')
+    (v_typNf : typNf Gamma v' ty)
+    : typNf Gamma v ty
+  where "Gamma '⊢' M '⇇' A" := (typNf Gamma M A).
+
+Fixpoint eval_typ (Gamma : ctx L) (ty : typ L) : trm L -> Set :=
+  match ty with
+  | bty _ b => fun M =>
+    B.sig (trm L) (fun N => Gamma ⊢ N ⇉ bty _ b /\ betaStar M N)
+  | (ty1 -> ty2)%typ => fun M =>
+    forall N, forall Gamma', le_ctx Gamma Gamma' -> eval_typ Gamma' ty1 N -> eval_typ Gamma' ty2 (App_trm M N)
   end.
 
-Definition interpret_ctx (Gamma : ctx L) (Delta : ctx L) : eval_ctx Gamma Delta -> subst L -> Prop :=
-  fun rho : eval_ctx Gamma Delta => fun gamma : subst L =>
-  forall x : name, forall ty : typ L, forall LOOKUP : Lookup x ty Gamma, interpret_typ Delta ty (rho x ty LOOKUP) (gamma x).
+(*
+Fixpoint reflect (Gamma : ctx L) (ty : typ L) {struct ty} : forall e, typNe Gamma e ty -> eval_typ Gamma ty e
+with reify (Gamma : ctx L) (ty : typ L) {struct ty} : forall e, eval_typ Gamma ty e -> typNf Gamma e ty.
+Proof.
+Admitted.
+*)
 
-End Soundness_of_NbE.
+Definition eval_ctx (Gamma : ctx L) (Delta : ctx L) : subst L -> Set :=
+  fun gamma => forall x, forall ty, Lookup x ty Delta -> eval_typ Gamma ty (gamma x).
+
+Definition semanticTyping (Gamma : ctx L) (e : trm L) (ty : typ L) : Set :=
+  forall Delta, forall gamma, eval_ctx Delta Gamma gamma -> eval_typ Delta ty (subst_trm gamma e).
+
+(*
+Theorem semanticTyping_sound Gamma e ty
+  (TYPING : Typing Gamma e ty)
+  : semanticTyping Gamma e ty.
+Proof.
+Admitted.
+*)
+
+End WEAK_NORMALISATION.
 
 End STLC_META.
 
